Fix compile errors

src/lang/Memory.v
@@ -1489,4 +1489,17 @@ Module Memory.
     exploit Cell.remove_exists; eauto. i. des.
     eexists. econs. eauto.
   Qed.
+
+  Definition nonsynch_loc (loc:Loc.t) (mem:t): Prop :=
+    forall f t msg (GET: get loc t mem = Some (f, msg)),
+      msg.(Message.released) = None.
+
+  Definition nonsynch (mem:t): Prop :=
+    forall loc, nonsynch_loc loc mem.
+
+  Lemma bot_nonsynch_loc loc: nonsynch_loc loc Memory.bot.
+  Proof. ii. rewrite bot_get in *. congr. Qed.
+
+  Lemma bot_nonsynch: nonsynch Memory.bot.
+  Proof. ii. eapply bot_nonsynch_loc. eauto. Qed.
 End Memory.
